%!TEX program = xelatex
\title          {Logic in Computer Science - Assignment 1}
\author         {李鹏达 10225101460}
\date{}

\documentclass{article}
\usepackage{../boxproof}
\usepackage{a4wide}
\usepackage{ctex}
% \usepackage{daymonthyear}

\def\meta#1{\mbox{$\langle\hbox{#1}\rangle$}}
\def\macrowitharg#1#2{{\tt\string#1\bra\meta{#2}\ket}}

{\escapechar-1 \xdef\bra{\string\{}\xdef\ket{\string\}}}

\showboxbreadth 999
\showboxdepth 999
\tracingoutput 1


\let\imp\to

\def\premise{\mathrm{premise}}
\def\assumption{\mathrm{assumption}}
\def\MT{\mathrm{MT\ }}
\def\LEM{\mathrm{LEM}}
\def\intro{\mathrm{i\ }}
\def\elim{\mathrm{e\ }}
\def\introa{\mathrm{i_1\ }}
\def\elima{\mathrm{e_1\ }}
\def\introb{\mathrm{i_2\ }}
\def\elimb{\mathrm{e_2\ }}

\def\lt{<}
\def\eqdef{=}

\def\eps{\mathrel{\epsilon}}
\def\biimplies{\leftrightarrow}
\def\flt#1{\mathrel{{#1}^\flat}}
\def\setof#1{{\left\{{#1}\right\}}}
\let\implies\to
\def\KK{{\mathsf K}}
\let\squashmuskip\relax


\def\pre{\premise}
\def\ass{\assumption}
\def\andea{\land\elima}
\def\andeb{\land\elimb}
\def\andi{\land\intro}
\def\toe{\to\elim}
\def\toi{\to\intro}
\def\ore{\lor\elim}
\def\ore{\lor\elim}
\def\oria{\lor\introa}
\def\orib{\lor\introb}
\def\nege{\neg\elim}
\def\negi{\neg\intro}

\def\tt{\!-\!}

%=======================================================================
\begin{document}
\maketitle
%=======================================================================
\noindent Prove the following Theorems with natural deduction:
\\[1em]
(1) $p \to q, r \to s \vdash p \land r \to q \land s$

$$
\begin{proofbox}
\: p \to q \= \pre \\
\: r \to s \= \pre \\
\[
    \: p \land r \= \ass \\
    \: p \=  \andea 3 \\
    \: r \= \andeb 3 \\
    \: q \=  \toe 1,4 \\
    \: s \=  \toe 2,5 \\
    \: q \land s \= \andi 4,5 \\
\]
\: p \land r \to q \land s \= \toi 3\tt8 \\
\end{proofbox}
$$
\\[1em]
(2) $\neg (p \land q) \vdash \neg q \lor \neg p$

$$
\begin{proofbox}
\: \neg (p \land q) \= \pre \\
\: q \land \neg q \= \LEM \\
\[
    \: \neg q \= \ass \\
    \: \neg q \lor \neg p \= \oria 3 \\
\]
\[
    \: q \= \ass \\
    \[
        \: p \= \ass \\
        \: p \land q \= \andi 5,6 \\
        \: \bot \= \nege 1,7 \\
    \]
    \: \neg p \= \negi 6\tt8 \\
    \: \neg q \lor \neg p \= \orib 9 \\
\]
\: \neg q \lor \neg p \= \ore 2,3\tt4,5\tt10
\end{proofbox}
$$
\\[1em]
(3) $p \to (q \lor r), q \to s, r \to s \vdash p \to s$

$$\begin{proofbox}
\: p \to (q \lor r) \= \pre \\
\: q \to s \= \pre \\
\: r \to s \= \pre \\
\[
\: p \= \ass \\
\: q \lor r \= \toe 1,4 \\
\[
    \: q \= \ass \\
    \: s \= \toe 2,6 \\
\]
\[
    \: r \= \ass \\
    \: s \= \toe 3,8 \\
\]
\: s \= \ore 5,6\tt7,8\tt9 \\
\]
\: p \to s \= \toi 4\tt10 \\
\end{proofbox}$$
\end{document}

